cleaned up embedding fsim

examples/CompCertIntSpec.v
@@ -23,7 +23,7 @@ Import ISpec.
 (** ** Embed Labelled Tranition Systems *)
 Section LTS.
 
-  Context {liA liB state} (L: lts liA liB state).
+  Context {liA liB} (L: semantics liA liB).
 
   (** *** Demonic Interpretation *)
   Section DEM.
@@ -44,58 +44,61 @@ Section LTS.
       transition does not finish within the number of steps, it
       crashes. Eventually, we use an angelic choice over the number of steps. *)
 
-    Fixpoint dem_lts_spec' (n: nat) (s: state): ispec liA (reply liB) :=
+    Fixpoint dem_lts_spec' (n: nat) (s: state L) se: ispec liA (reply liB) :=
       match n with
       | O => bot
       | S n =>
-          _ <- assert (safe L s);
+          _ <- assert (safe (L se) s);
           (* internal step *)
-          (inf { s' | Step L s E0 s' }, dem_lts_spec' n s') &&
+          (inf { s' | Step (L se) s E0 s' }, dem_lts_spec' n s' se) &&
           (* external call *)
-          (inf { q | at_external L s q },
-           r <- query_int q;
-           _ <- assert (exists s', after_external L s r s');
-           inf { s' | after_external L s r s' }, dem_lts_spec' n s') &&
+          (inf { q | at_external (L se) s q },
+           r <- query_int q se;
+           _ <- assert (exists s', after_external (L se) s r s');
+           inf { s' | after_external (L se) s r s' }, dem_lts_spec' n s' se) &&
           (* final state *)
-          (inf { r | final_state L s r }, ret r)
+          (inf { r | final_state (L se) s r }, ret r)
       end.
 
     Definition dem_lts_spec: subst liA liB :=
-      fun _ '(li_sig q) => sup n,
-        _ <- assert (exists s, initial_state L q s);
-        inf { s | initial_state L q s }, dem_lts_spec' n s.
+      fun _ '(li_sig q se) => sup n,
+        _ <- assert (exists s, initial_state (L se) q s);
+        inf { s | initial_state (L se) q s }, dem_lts_spec' n s se.
 
   End DEM.
 
   (** *** Angelic Semantics *)
   Section ANG.
 
-    Fixpoint ang_lts_spec' (n: nat) (s: state): ispec liA (reply liB) :=
+    Fixpoint ang_lts_exec (n: nat) (s: state L) se: ispec liA (reply liB) :=
       match n with
       | O => bot
       | S n =>
           (* internal step *)
-          (sup { s' | Star L s E0 s' }, ang_lts_spec' n s') ||
+          (sup { s' | Star (L se) s E0 s' }, ang_lts_exec n s' se) ||
           (* external call *)
-          (sup { q | at_external L s q },
-           r <- query_int q;
-           sup { s' | after_external L s r s' }, ang_lts_spec' n s') ||
+          (sup { q | at_external (L se) s q },
+           r <- query_int q se;
+           sup { s' | after_external (L se) s r s' }, ang_lts_exec n s' se) ||
           (* final step *)
-          (sup { r | final_state L s r }, ret r)
+          (sup { r | final_state (L se) s r }, ret r)
       end.
 
-    Definition ang_lts_spec: subst liA liB :=
-      fun _ '(li_sig q) => sup n,
-        sup { s | initial_state L q s }, ang_lts_spec' n s.
+    Definition ang_lts_spec' sk: subst liA liB :=
+      fun _ '(li_sig q se) =>
+        _ <- assert (Genv.valid_for sk se);
+        sup n, sup { s | initial_state (L se) q s }, ang_lts_exec n s se.
+
+    Definition ang_lts_spec: subst liA liB := ang_lts_spec' (skel L).
 
     (** Executing one step in the FCD specification *)
-    Lemma lts_spec_step s:
-      sup n, ang_lts_spec' n s =
-        (sup { s' | Star L s E0 s' }, sup n, ang_lts_spec' n s') ||
-        (sup { q | at_external L s q },
-          r <- query_int q;
-         sup { s' | after_external L s r s' }, sup n, ang_lts_spec' n s') ||
-        (sup { r | final_state L s r }, ret r).
+    Lemma lts_spec_step s se:
+      sup n, ang_lts_exec n s se =
+        (sup { s' | Star (L se) s E0 s' }, sup n, ang_lts_exec n s' se) ||
+        (sup { q | at_external (L se) s q },
+          r <- query_int q se;
+         sup { s' | after_external (L se) s r s' }, sup n, ang_lts_exec n s' se) ||
+        (sup { r | final_state (L se) s r }, ret r).
     Proof.
       apply antisymmetry.
       - apply sup_iff. intros i.
@@ -152,48 +155,222 @@ Section LTS.
     behavior, i.e. when the LTS is deterministic *)
   Section DET.
     Context (se: Genv.symtbl).
-    Hypothesis DET: lts_determinate L se.
+    Hypothesis DET: lts_determinate (L se) se.
 
     Lemma det_lts_spec_equiv:
       ang_lts_spec = dem_lts_spec.
-    Proof.
-      apply antisymmetry.
-      - intros ? [q]. cbn. apply sup_lub. intros i.
-        unfold assert.
-    Abort.
+    Proof. Abort.
 
   End DET.
 
-  (* Definitions for defining the embedding through the play instead of
-     interaction primitives. Not used for now *)
-  (* Inductive state_exec: state -> query liA + reply liB -> Prop :=
-  | state_exec_step s s' e:
-      Step L s E0 s' ->
-      state_exec s' e ->
-      state_exec s e
-  | state_exec_final s r:
-      final_state L s r ->
-      state_exec s (inr r)
-  | state_exec_external s q:
-      at_external L s q ->
-      state_exec s (inl q).
-
-  Inductive lts_play: state -> play liA (reply liB) -> Prop :=
-  | lts_play_step s s' p:
-    Step L s E0 s' ->
-    lts_play s' p ->
-    lts_play s p
-  | lts_play_ret s r:
-    final_state L s r ->
-    lts_play s (pret r)
-  | lts_play_query s q r (p: play liA (reply liB)) s':
-    lts_play s' p ->
-    at_external L s q ->
-    after_external L s r s' ->
-    lts_play s (pcons (li_sig q) r p). *)
-
 End LTS.
 
+Require Import CAL.
+
+(** The skeleton is used for choosing a compatible symbol table. So a larger
+  skeleton accepts less symbol tables and thus leads to less behavior. *)
+Instance skel_order_proper {liA liB} (L: semantics liA liB):
+  Proper (Linking.linkorder --> ref) (ang_lts_spec' L).
+Proof.
+  intros sk1 sk2 Hsk. intros k [qb se]. cbn.
+  apply assert_l. intros Hv.
+  apply assert_r. reflexivity.
+  eapply Genv.valid_for_linkorder; eauto.
+Qed.
+
+(* Note: it's hard to imply the [esig] from the context, since
+   higher-order unification is generally difficult, i.e. to imply [E] from [E X] *)
+
+Local Opaque normalize_rc.
+
+(** ** Monotonicity of Embedding *)
+Section SEM.
+
+  Context {liA1 liA2} (ccA: callconv liA1 liA2).
+  Context {liB1 liB2} (ccB: callconv liB1 liB2).
+  Context (L1: semantics liA1 liB1) (L2: semantics liA2 liB2).
+  Variable (sk: AST.program unit unit).
+  Hypothesis HSK: Linking.linkorder (skel L1) sk.
+  Hypothesis FSIM: forward_simulation ccA ccB L1 L2.
+
+  Lemma ang_fsim_embed' :
+    ang_lts_spec' L1 sk [= (right_arrow (cc_rc ccB)) @ ang_lts_spec' L2 sk @ (left_arrow (cc_rc ccA)).
+  Proof.
+    intros k [qb1 se1]. unfold compose. cbn.
+    apply assert_l. intros Hv1.
+    apply sup_iff. intros steps.
+    apply sup_iff. intros [s H1]. cbn.
+    unfold rc_adj_right. inf_intro a. inf_intro [qb2 se2].
+    inf_intro [Rrb Hrb]. rc_inversion Hrb. depsubst.
+    rename H5 into Hse. rename H6 into Hqb. rename w into wB.
+    clear Hrel. rename Hsub into HRrb.
+    destruct FSIM as [[? ? match_states Hskeq Hfp Hlts Hwf]].
+    clear FSIM. rename Hlts into FSIM.
+    assert (Hsk1: Genv.valid_for (skel L1) se1).
+    { eapply Genv.valid_for_linkorder; eauto. }
+    specialize (FSIM se1 se2 wB Hse Hsk1).
+    intm.
+    assert (Hv2: Genv.valid_for sk se2).
+    { eapply match_senv_valid_for; eauto. }
+    eapply @assert_true in Hv2. setoid_rewrite Hv2.
+    clear Hv1 Hv2 Hskeq.
+    intm. sup_mor. apply (sup_at steps).
+    edestruct (fsim_match_initial_states FSIM) as (i & s2 & H2 & Hs); eauto.
+    sup_mor. eapply (fsup_at s2). apply H2.
+    clear H1 H2 Hqb. revert i s s2 Hs.
+    induction steps; eauto using bot_lb.
+    intros i s1 s2 Hs. cbn.
+    repeat apply join_lub.
+    - sup_intro [s1' Hstep]. apply join_l. apply join_l.
+      assert (exists i s2', Star (L2 se2) s2 E0 s2' /\ match_states se1 se2 wB i s1' s2') as (i' & s2' & Hstep2 & Hs').
+      {
+        revert i s2 Hs. pattern s1, s1'. eapply star_E0_ind; eauto; clear s1 s1' Hstep.
+        - intros s1 i s2 Hs. exists i, s2; split; eauto using star_refl.
+        - intros s1 s1' s1'' Hstep1 IHstar i s2 Hs.
+          edestruct (simulation_star FSIM) as (i' & s2' & Hstep2 & Hs'); eauto using star_one.
+          specialize (IHstar _ _ Hs') as (i'' & s2'' & Hstep2' & Hs'').
+          eexists i'', s2''. split; eauto.
+          eapply star_trans; eauto.
+      }
+      sup_mor. eapply (fsup_at s2'). apply Hstep2.
+      specialize (IHsteps _ _ _ Hs'). apply IHsteps.
+    - sup_intro [qa1 H1]. apply join_l. apply join_r.
+      edestruct @fsim_match_external as (w & qa2 & H2 & Hqa & Hse' & Hrx); eauto.
+      sup_mor. eapply (fsup_at qa2). apply H2.
+      unfold query_int. intm. unfold rc_adj_left at 3.
+      sup_mor. eapply sup_at.
+      sup_mor. eapply (sup_at (li_sig qa1 se1)).
+      sup_mor. eapply (fsup_at (match_reply ccA w)).
+      { rc_econstructor; eauto. }
+      intm. sup_mor. apply sup_iff. intros [ ra1 | ].
+      + fcd_simpl. apply join_lub.
+        * apply (sup_at None). fcd_simpl. reflexivity.
+        * apply (sup_at (Some ra1)).
+          fcd_simpl. apply join_r.
+          inf_intro [ra2 Hr]. intm.
+          sup_intro [s' H1'].
+          specialize (Hrx _ _ _ Hr H1') as (i' & s2' & H2' & Hs').
+          eapply (fsup_at s2'). apply H2'.
+          specialize (IHsteps _ _ _ Hs').
+          rewrite IHsteps. reflexivity.
+      + apply (sup_at None). fcd_simpl. reflexivity.
+    - sup_intro [rb1 H1]. apply join_r.
+      edestruct @fsim_match_final_states as (rb2 & H2 & Hr); eauto.
+      sup_mor. apply (fsup_at rb2). apply H2.
+      intm. sup_mor.
+      apply (fsup_at rb1). apply HRrb. apply Hr.
+      intm. reflexivity.
+  Qed.
+
+End SEM.
+
+Lemma ang_fsim_embed {liA1 liA2 liB1 liB2} ccA ccB
+      (L1: semantics liA1 liB1) (L2: semantics liA2 liB2):
+  forward_simulation ccA ccB L1 L2 ->
+  ang_lts_spec L1 [= (right_arrow (cc_rc ccB)) @ ang_lts_spec L2 @ (left_arrow (cc_rc ccA)).
+Proof.
+  intros FSIM. destruct FSIM as [[]].
+  unfold ang_lts_spec. rewrite <- fsim_skel.
+  apply ang_fsim_embed'.
+  apply Linking.linkorder_refl.
+  constructor. econstructor; eauto.
+Qed.
+
+Require Import compcert.common.CategoricalComp.
+
+(** ** Functoriality of the embedding *)
+(** We prove the embedding preserves composition, i.e. ⟦L1⟧ ∘ ⟦L2⟧ ⊑ ⟦L1 ∘ L2⟧. *)
+Section COMP.
+
+  Context {liA liB liC} (L1: semantics liB liC) (L2: semantics liA liB).
+  Context {L} (COMP: comp_semantics L1 L2 = Some L).
+  Variable (sk: AST.program unit unit).
+  Hypothesis HSK: Linking.linkorder (skel L) sk.
+
+  Lemma comp_embed':
+    ang_lts_spec' L1 sk @ ang_lts_spec' L2 sk [= ang_lts_spec' L sk.
+  Proof.
+    Local Opaque comp_semantics'.
+    intros _ [qc se]. unfold comp_semantics, option_map in COMP.
+    destruct Linking.link eqn: Hlk; try congruence. inv COMP.
+    unfold ISpec.compose. unfold ang_lts_spec' at 2.
+    sup_mor. sup_mor. apply sup_iff. intros Hsk.
+    apply (sup_at Hsk). intm. sup_intro steps1.
+    sup_intro [s1 Hinit]. unfold fsup. rewrite sup_sup.
+    exploit @comp_initial_state_intro. eapply Hinit. intro Hinit'.
+    eapply (sup_at (exist _ (st1 _ _ s1) Hinit')). cbn.
+    clear Hinit Hinit'. revert s1. induction steps1.
+    - intros s. apply (sup_at 0%nat). cbn.
+      rewrite Sup.mor_bot. reflexivity.
+    - intros s1. cbn. rewrite !Sup.mor_join. repeat apply join_lub.
+      + sup_intro [s1' Hstep1].
+        exploit @star_internal1. apply Hstep1. intros Hstep.
+        specialize (IHsteps1 s1'). etransitivity. apply IHsteps1.
+        apply sup_iff. intros steps. apply (sup_at (S steps)).
+        cbn. apply join_l. apply join_l.
+        eapply fsup_at. apply Hstep. reflexivity.
+      + sup_intro [qb1 Hext1]. unfold query_int. intm.
+        sup_intro steps2. sup_intro [s2 Hinit2].
+        rewrite lts_spec_step. apply join_l. apply join_l.
+        eapply fsup_at. apply star_one. eapply step_push; eauto.
+
+        clear Hext1 Hinit2. revert s2. induction steps2; intros s2; cbn.
+        * rewrite Sup.mor_bot. apply bot_lb.
+        * rewrite !Sup.mor_join. repeat apply join_lub.
+          -- sup_intro [s2' H2]. specialize (IHsteps2 s2').
+             etransitivity. apply IHsteps2.
+             apply sup_iff. intros steps. apply (sup_at (S steps)). cbn.
+             apply join_l. apply join_l.
+             eapply fsup_at. apply star_internal2; eauto. reflexivity.
+          -- sup_intro [qa Hext2]. unfold query_int. intm.
+             assert (Hcrash: (FCD.emb (@pmove (sig liA) _ _ (li_sig qa se))) [=
+                               sup n : nat, ang_lts_exec ((comp_semantics' L1 L2 p) ) n (st2 L1 L2 s1 s2) se).
+             {
+               apply (sup_at 1%nat). cbn. apply join_l. apply join_r.
+               eapply fsup_at. econstructor; eauto.
+               unfold query_int. sup_mor. apply (sup_at None).
+               fcd_simpl. reflexivity.
+             }
+             sup_intro [ra|].
+             ++ fcd_simpl. apply join_lub.
+                ** apply Hcrash.
+                ** sup_intro [s2' Haft].
+                   specialize (IHsteps2 s2').
+                   rewrite IHsteps2. clear IHsteps2.
+                   sup_intro steps. apply (sup_at (S steps)). cbn.
+                   apply join_l. apply join_r.
+                   eapply fsup_at. econstructor; eauto.
+                   unfold query_int. sup_mor. apply (sup_at (Some ra)).
+                   fcd_simpl. apply join_r.
+                   sup_mor. eapply (fsup_at (st2 _ _ s1 s2')). now constructor.
+                   apply ext_proper_ref; try typeclasses eauto.
+                   intros c. reflexivity. reflexivity.
+             ++ fcd_simpl. apply Hcrash.
+          -- sup_intro [rb Hfinal2]. intm.
+             sup_intro [s1' Haft1].
+             specialize (IHsteps1 s1').
+             etransitivity. apply IHsteps1.
+             apply sup_iff. intros steps. apply (sup_at (S steps)).
+             cbn. apply join_l. apply join_l.
+             eapply fsup_at. apply star_one. eapply step_pop; eauto.
+             reflexivity.
+      + sup_intro [rc Hfinal1]. fcd_simpl.
+        apply (sup_at 1%nat). cbn. apply join_r.
+        eapply fsup_at. constructor; eauto. reflexivity.
+  Qed.
+
+End COMP.
+
+Lemma comp_embed {liA liB liC} (L1: semantics liB liC) (L2: semantics liA liB) L:
+  comp_semantics L1 L2 = Some L ->
+  ang_lts_spec' L1 (skel L) @ ang_lts_spec' L2 (skel L) [= ang_lts_spec L.
+Proof.
+  intros COMP. unfold ang_lts_spec.
+  rewrite <- (comp_embed' _ _ COMP). 2: apply Linking.linkorder_refl.
+  reflexivity.
+Qed.
+
+(*
 (** ** Embed Calling Conventions *)
 Section CC.
 
@@ -381,362 +558,4 @@ Section CC_SE.
     |}.
 
 End CC_SE.
-
-(* Note: it's hard to imply the [esig] from the context, since
-   higher-order unification is generally difficult, i.e. to imply [E] from [E X] *)
-
-(** ** Monotonicity of Embedding *)
-Section FSIM.
-
-  Context {liA1 liA2} (ccA: callconv liA1 liA2).
-  Context {liB1 liB2} (ccB: callconv liB1 liB2).
-  Context (se1 se2: Genv.symtbl).
-  Context {state1 state2: Type}.
-  Context (L1: lts liA1 liB1 state1) (L2: lts liA2 liB2 state2).
-  Context (index: Type) (order: index -> index -> Prop)
-          (match_states: Genv.symtbl -> Genv.symtbl -> ccworld ccB ->index -> state1 -> state2 -> Prop).
-  Hypothesis FSIM:
-    forall wB, fsim_properties ccA ccB se1 se2 wB L1 L2 index order (match_states se1 se2 wB).
-
-  Lemma ang_fsim_embed:
-    ang_lts_spec L1 [= (cc_right ccB) @ ang_lts_spec L2 @ (cc_left ccA).
-  Proof.
-    intros k [qb1]. unfold ISpec.compose.
-    unfold ang_lts_spec at 1.
-    apply sup_iff. intros steps.
-    apply sup_iff. intros [s H1]. cbn.
-    unfold finf. rewrite Inf.mor.
-    apply inf_iff. intros wB. specialize (FSIM wB).
-    rewrite Inf.mor.
-    apply inf_iff. intros [qb2 Hqb].
-    unfold query_int. intm.
-    setoid_rewrite Sup.mor.
-    setoid_rewrite apply_ret.
-    setoid_rewrite Sup.mor.
-    unfold bind. repeat setoid_rewrite Sup.mor.
-    apply sup_at with (i := steps).
-    edestruct (fsim_match_initial_states FSIM) as (i & s2 & H2 & Hs); eauto.
-    eapply (sup_at (exist _ s2 H2)). cbn.
-    clear H1 H2 Hqb. revert i s s2 Hs.
-    induction steps; eauto using bot_lb.
-    intros i s1 s2 Hs. cbn.
-    repeat apply join_lub.
-    - apply sup_iff. intros [s1' Hstep]. cbn.
-      rewrite !Sup.mor_join.
-      apply join_l. apply join_l.
-      assert (exists i s2', Star L2 s2 E0 s2' /\ match_states se1 se2 wB i s1' s2') as (i' & s2' & Hstep2 & Hs').
-      {
-        revert i s2 Hs. pattern s1, s1'. eapply star_E0_ind; eauto; clear s1 s1' Hstep.
-        - intros s1 i s2 Hs. exists i, s2; split; eauto using star_refl.
-        - intros s1 s1' s1'' Hstep1 IHstar i s2 Hs.
-          edestruct (simulation_star FSIM) as (i' & s2' & Hstep2 & Hs'); eauto using star_one.
-          specialize (IHstar _ _ Hs') as (i'' & s2'' & Hstep2' & Hs'').
-          eexists i'', s2''. split; eauto.
-          eapply star_trans; eauto.
-      }
-      repeat setoid_rewrite Sup.mor.
-      eapply (sup_at (exist _ s2' Hstep2)). cbn.
-      specialize (IHsteps _ _ _ Hs'). apply IHsteps.
-    - apply sup_iff. intros [qa1 H1]. cbn.
-      rewrite !Sup.mor_join.
-      apply join_l. apply join_r.
-      edestruct @fsim_match_external as (w & qa2 & H2 & Hqa & _ & Hrx); eauto.
-      setoid_rewrite Sup.mor.
-      setoid_rewrite Sup.mor.
-      eapply (sup_at (exist _ qa2 H2)). cbn.
-      rewrite apply_bind. unfold query_int.
-      rewrite apply_int_r.
-      unfold bind. unfold cc_left at 2.
-      repeat setoid_rewrite Sup.mor.
-      eapply (sup_at w).
-      eapply (sup_at (exist _ qa1 Hqa)). cbn.
-      unfold query_int. unfold bind.
-      apply sup_iff. intros [ra1|].
-      + rewrite FCD.ext_ana. cbn.
-        apply join_lub.
-        * apply (sup_at (Some ra1)).
-          rewrite FCD.ext_ana. cbn.
-          rewrite !Sup.mor_join. apply join_l.
-          rewrite FCD.ext_ana. cbn.
-          rewrite FCD.ext_ana. cbn. reflexivity.
-        * apply (sup_at (Some ra1)).
-          rewrite FCD.ext_ana. cbn.
-          rewrite !Sup.mor_join. apply join_r.
-          repeat setoid_rewrite Inf.mor.
-          apply inf_iff. intros [ra2 Hr]. cbn.
-          unfold ret at 2. cbn.
-          repeat setoid_rewrite FCD.ext_ana. cbn.
-          rewrite !Sup.mor_join. apply join_r.
-          setoid_rewrite Sup.mor.
-          apply sup_iff. intros [s' H1'].
-          specialize (Hrx _ _ _ Hr H1') as (i' & s2' & H2' & Hs'). cbn.
-          setoid_rewrite Sup.mor.
-          apply (sup_at (exist _ s2' H2')). cbn.
-          specialize (IHsteps _ _ _ Hs').
-          etransitivity.
-          -- instantiate (1 := FCD.ext _ _). rstep. reflexivity.
-          -- rewrite IHsteps. unfold apply.
-             rewrite FCD.ext_ext. unfold t. rewrite FCD.ext_ext.
-             eapply ext_proper_ref'.
-             ++ split. intros a b Hab. rstep. now apply pbind_mor.
-             ++ split. intros a b Hab. repeat rstep. now constructor.
-             ++ intros x. rewrite FCD.ext_ana. cbn. apply join_r. reflexivity.
-      + rewrite FCD.ext_ana. cbn.
-        apply (sup_at None).
-        repeat (setoid_rewrite FCD.ext_ana; cbn).
-        reflexivity.
-    - apply sup_iff. intros [rb1 H1]. cbn.
-      rewrite !Sup.mor_join. apply join_r.
-      edestruct @fsim_match_final_states as (rb2 & H2 & Hr); eauto.
-      repeat setoid_rewrite Sup.mor.
-      apply (sup_at (exist _ rb2 H2)). cbn.
-      rewrite apply_ret.
-      unfold ret at 3. rewrite FCD.ext_ana. cbn.
-      apply (sup_at (exist _ rb1 Hr)). cbn.
-      reflexivity.
-  Qed.
-
-End FSIM.
-
-Section FSIM.
-
-  Context {liA1 liA2} (ccA: callconv liA1 liA2).
-  Context {liB1 liB2} (ccB: callconv liB1 liB2).
-  Context (se1 se2: Genv.symtbl).
-  Context {state1 state2: Type}.
-  Context (L1: lts liA1 liB1 state1) (L2: lts liA2 liB2 state2).
-  Context (index: Type) (order: index -> index -> Prop)
-          (match_states: Genv.symtbl -> Genv.symtbl -> ccworld ccB ->index -> state1 -> state2 -> Prop).
-  Hypothesis FSIM:
-    forall wB, match_senv ccB wB se1 se2 ->
-      fsim_properties ccA ccB se1 se2 wB L1 L2 index order (match_states se1 se2 wB).
-
-  Lemma ang_fsim_embed_se:
-    ang_lts_spec L1 [= (cc_r ccB se1 se2) @ ang_lts_spec L2 @ (cc_l ccA se1 se2).
-  Proof.
-    intros k [qb1]. unfold ISpec.compose.
-    unfold ang_lts_spec at 1.
-    apply sup_iff. intros steps.
-    apply sup_iff. intros [s H1]. cbn.
-    unfold finf. rewrite Inf.mor.
-    apply inf_iff. intros [ wB Hse ]. specialize (FSIM wB Hse).
-    rewrite Inf.mor. apply inf_iff. intros [qb2 Hqb].
-    unfold query_int. intm.
-    setoid_rewrite Sup.mor.
-    setoid_rewrite apply_ret.
-    setoid_rewrite Sup.mor.
-    unfold bind. repeat setoid_rewrite Sup.mor.
-    apply sup_at with (i := steps).
-    edestruct (fsim_match_initial_states FSIM) as (i & s2 & H2 & Hs); eauto.
-    eapply (sup_at (exist _ s2 H2)). cbn.
-    clear H1 H2 Hqb. revert i s s2 Hs.
-    induction steps; eauto using bot_lb.
-    intros i s1 s2 Hs. cbn.
-    repeat apply join_lub.
-    - apply sup_iff. intros [s1' Hstep]. cbn.
-      rewrite !Sup.mor_join.
-      apply join_l. apply join_l.
-      assert (exists i s2', Star L2 s2 E0 s2' /\ match_states se1 se2 wB i s1' s2') as (i' & s2' & Hstep2 & Hs').
-      {
-        revert i s2 Hs. pattern s1, s1'. eapply star_E0_ind; eauto; clear s1 s1' Hstep.
-        - intros s1 i s2 Hs. exists i, s2; split; eauto using star_refl.
-        - intros s1 s1' s1'' Hstep1 IHstar i s2 Hs.
-          edestruct (simulation_star FSIM) as (i' & s2' & Hstep2 & Hs'); eauto using star_one.
-          specialize (IHstar _ _ Hs') as (i'' & s2'' & Hstep2' & Hs'').
-          eexists i'', s2''. split; eauto.
-          eapply star_trans; eauto.
-      }
-      repeat setoid_rewrite Sup.mor.
-      eapply (sup_at (exist _ s2' Hstep2)). cbn.
-      specialize (IHsteps _ _ _ Hs'). apply IHsteps.
-    - apply sup_iff. intros [qa1 H1]. cbn.
-      rewrite !Sup.mor_join.
-      apply join_l. apply join_r.
-      edestruct @fsim_match_external as (w & qa2 & H2 & Hqa & Hse' & Hrx); eauto.
-      setoid_rewrite Sup.mor.
-      setoid_rewrite Sup.mor.
-      eapply (sup_at (exist _ qa2 H2)). cbn.
-      rewrite apply_bind. unfold query_int.
-      rewrite apply_int_r.
-      unfold bind. unfold cc_l at 2.
-      repeat setoid_rewrite Sup.mor.
-      eapply (sup_at (exist _ w Hse')). cbn.
-      eapply (sup_at (exist _ qa1 Hqa)). cbn.
-      unfold query_int. unfold bind.
-      apply sup_iff. intros [ra1|].
-      + rewrite FCD.ext_ana. cbn.
-        apply join_lub.
-        * apply (sup_at (Some ra1)).
-          rewrite FCD.ext_ana. cbn.
-          rewrite !Sup.mor_join. apply join_l.
-          rewrite FCD.ext_ana. cbn.
-          rewrite FCD.ext_ana. cbn. reflexivity.
-        * apply (sup_at (Some ra1)).
-          rewrite FCD.ext_ana. cbn.
-          rewrite !Sup.mor_join. apply join_r.
-          repeat setoid_rewrite Inf.mor.
-          apply inf_iff. intros [ra2 Hr]. cbn.
-          unfold ret at 2. cbn.
-          repeat setoid_rewrite FCD.ext_ana. cbn.
-          rewrite !Sup.mor_join. apply join_r.
-          setoid_rewrite Sup.mor.
-          apply sup_iff. intros [s' H1'].
-          specialize (Hrx _ _ _ Hr H1') as (i' & s2' & H2' & Hs'). cbn.
-          setoid_rewrite Sup.mor.
-          apply (sup_at (exist _ s2' H2')). cbn.
-          specialize (IHsteps _ _ _ Hs').
-          etransitivity.
-          -- instantiate (1 := FCD.ext _ _). rstep. reflexivity.
-          -- rewrite IHsteps. unfold apply.
-             rewrite FCD.ext_ext. unfold t. rewrite FCD.ext_ext.
-             eapply ext_proper_ref'.
-             ++ split. intros a b Hab. rstep. now apply pbind_mor.
-             ++ split. intros a b Hab. repeat rstep. now constructor.
-             ++ intros x. rewrite FCD.ext_ana. cbn. apply join_r. reflexivity.
-      + rewrite FCD.ext_ana. cbn.
-        apply (sup_at None).
-        repeat (setoid_rewrite FCD.ext_ana; cbn).
-        reflexivity.
-    - apply sup_iff. intros [rb1 H1]. cbn.
-      rewrite !Sup.mor_join. apply join_r.
-      edestruct @fsim_match_final_states as (rb2 & H2 & Hr); eauto.
-      repeat setoid_rewrite Sup.mor.
-      apply (sup_at (exist _ rb2 H2)). cbn.
-      rewrite apply_ret.
-      unfold ret at 3. rewrite FCD.ext_ana. cbn.
-      apply (sup_at (exist _ rb1 Hr)). cbn.
-      reflexivity.
-  Qed.
-
-End FSIM.
-
-Section SEM.
-
-  Context {liA1 liA2} (ccA: callconv liA1 liA2).
-  Context {liB1 liB2} (ccB: callconv liB1 liB2).
-  Context (L1: semantics liA1 liB1) (L2: semantics liA2 liB2).
-  Context (se1 se2: Genv.symtbl).
-
-  Hypothesis FSIM: forward_simulation ccA ccB L1 L2.
-  Hypothesis HSK: Genv.valid_for (skel L1) se1.
-
-  Lemma ang_fsim_embed':
-    ang_lts_spec (L1 se1) [= (cc_r ccB se1 se2) @ ang_lts_spec (L2 se2) @ (cc_l ccA se1 se2).
-  Proof.
-    pose proof (ang_fsim_embed_se ccA ccB).
-    destruct FSIM as [ [ ] ]. eapply H.
-    intros wB Hse. apply fsim_lts; eauto.
-  Qed.
-
-End SEM.
-
-Require Import compcert.common.CategoricalComp.
-
-(** ** Functoriality of the embedding *)
-(** We prove the embedding preserves composition, i.e. ⟦L1⟧ ∘ ⟦L2⟧ ⊑ ⟦L1 ∘ L2⟧ *)
-Section COMP.
-
-  Context {liA liB liC} (L1: semantics liB liC) (L2: semantics liA liB).
-  Context {L} (COMP: comp_semantics L1 L2 = Some L).
-
-  Lemma comp_embed se:
-    ang_lts_spec (L1 se) @ ang_lts_spec (L2 se) [= ang_lts_spec (L se).
-  Proof.
-    Local Opaque comp_semantics'.
-    intros _ [qc]. unfold comp_semantics, option_map in COMP.
-    destruct Linking.link; try congruence. inv COMP.
-    unfold ISpec.compose. unfold ang_lts_spec at 2.
-    rewrite Sup.mor. apply sup_iff. intros steps1.
-    setoid_rewrite Sup.mor. apply sup_iff.
-    intros [s1 Hinit]. cbn. unfold fsup. rewrite sup_sup.
-    exploit @comp_initial_state_intro. eapply Hinit. intro Hinit'.
-    eapply (sup_at (exist _ (st1 _ _ s1) Hinit')). cbn.
-    clear Hinit Hinit'. revert s1. induction steps1.
-    - intros s. apply (sup_at 0%nat). cbn.
-      rewrite Sup.mor_bot. reflexivity.
-    - intros s1. cbn. rewrite !Sup.mor_join. repeat apply join_lub.
-      + setoid_rewrite Sup.mor.
-        apply sup_iff. intros [s1' Hstep1]. cbn.
-        exploit @star_internal1. apply Hstep1. intros Hstep.
-        specialize (IHsteps1 s1'). etransitivity. apply IHsteps1.
-        apply sup_iff. intros steps. apply (sup_at (S steps)).
-        cbn. apply join_l. apply join_l.
-        eapply fsup_at. apply Hstep. reflexivity.
-      + setoid_rewrite Sup.mor. apply sup_iff.
-        intros [qb1 Hext1]. cbn.
-        rewrite apply_bind. unfold query_int.
-        rewrite apply_int_r. unfold bind. unfold ang_lts_spec at 2.
-        rewrite Sup.mor. setoid_rewrite Sup.mor.
-        apply sup_iff. intros steps2.
-        apply sup_iff. intros [s2 Hinit2]. cbn.
-        rewrite lts_spec_step.
-        apply join_l. apply join_l.
-        eapply fsup_at. apply star_one. eapply step_push; eauto.
-
-        clear Hext1 Hinit2. revert s2. induction steps2; intros s2; cbn.
-        * rewrite Sup.mor_bot. apply bot_lb.
-        * rewrite !Sup.mor_join. repeat apply join_lub.
-          -- setoid_rewrite Sup.mor. apply sup_iff.
-             intros [s2' H2]. cbn. specialize (IHsteps2 s2').
-             etransitivity. apply IHsteps2.
-             apply sup_iff. intros steps. apply (sup_at (S steps)). cbn.
-             apply join_l. apply join_l.
-             eapply fsup_at. apply star_internal2; eauto. reflexivity.
-          -- setoid_rewrite Sup.mor. apply sup_iff.
-             intros [qa Hext2]. cbn.
-             unfold bind. unfold query_int.
-             setoid_rewrite Sup.mor at 2. setoid_rewrite Sup.mor at 1.
-             apply sup_iff.
-             assert (Hcrash: (FCD.emb (@pmove (sig liA) _ _ qa)) [=
-                               sup n : nat, ang_lts_spec' ((comp_semantics' L1 L2 p) se) n (st2 L1 L2 s1 s2)).
-             {
-               apply (sup_at 1%nat). cbn.
-               apply join_l. apply join_r.
-               eapply fsup_at. econstructor; eauto.
-               unfold bind. unfold query_int.
-               setoid_rewrite Sup.mor. apply (sup_at None).
-               rewrite FCD.ext_ana. cbn. reflexivity.
-             }
-             intros [ra|].
-             ++ setoid_rewrite FCD.ext_ana. cbn.
-                rewrite Sup.mor_join. apply join_lub.
-                ** rewrite FCD.ext_ana. apply Hcrash.
-                ** setoid_rewrite Sup.mor at 2. rewrite Sup.mor.
-                   apply sup_iff. intros [s2' Haft]. cbn.
-                   pose proof @fmap_cons as fc. unfold bind in fc.
-                   rewrite fc. clear fc.
-                   apply join_lub.
-                   --- apply Hcrash.
-                   --- specialize (IHsteps2 s2').
-                       rewrite IHsteps2.
-                       rewrite Sup.mor. apply sup_iff. intros steps.
-                       apply (sup_at (S steps)). cbn.
-                       apply join_l. apply join_r.
-                       eapply fsup_at. econstructor; eauto.
-                       unfold bind. unfold query_int.
-                       setoid_rewrite Sup.mor. apply (sup_at (Some ra)).
-                       rewrite FCD.ext_ana. cbn. apply join_r.
-                       apply ext_proper_ref; try typeclasses eauto.
-                       intros c. reflexivity.
-                       eapply fsup_at. econstructor; eauto. reflexivity.
-             ++ rewrite FCD.ext_ana. cbn.
-                rewrite FCD.ext_ana. apply Hcrash.
-          -- setoid_rewrite Sup.mor. apply sup_iff.
-             intros [rb Hfinal2]. cbn.
-             unfold ret. rewrite FCD.ext_ana. cbn.
-             setoid_rewrite Sup.mor. apply sup_iff.
-             intros [s1' Haft1]. cbn.
-             specialize (IHsteps1 s1').
-             etransitivity. apply IHsteps1.
-             apply sup_iff. intros steps. apply (sup_at (S steps)).
-             cbn. apply join_l. apply join_l.
-             eapply fsup_at. apply star_one. eapply step_pop; eauto.
-             reflexivity.
-      + setoid_rewrite Sup.mor. apply sup_iff.
-        intros [rc Hfinal1]. cbn. unfold ret.
-        setoid_rewrite FCD.ext_ana. cbn.
-        apply (sup_at 1%nat). cbn. apply join_r.
-        eapply fsup_at. constructor; eauto. reflexivity.
-  Qed.
-
-End COMP.
+*)
